Inductive schemas worked! af_bind proofs complete

theories/ITree/Logic/AF.v
@@ -28,9 +28,49 @@ Local Open Scope ctl_scope.
 Local Open Scope itree_scope.
   
 (*| CTL logic lemmas on c/itrees |*)
-Section CtlITrees.
+Section BasicLemmas.
+  Context {E: Type} {HE: Encode E} {X: Type} (φ: X -> World E -> Prop).
+
+  Lemma af_tau: forall (t: itree E X) w φ,
+      <( t, w |= AF now φ )> -> 
+      <( {Tau t}, w |= AF (now φ) )>.
+  Proof.
+    intros.
+    unfold entailsF in H.
+    induction H.
+    - now next; left.
+    - Opaque entailsF.
+      destruct H0, H1; clear H H1.
+      destruct H0 as (t' & w' & TR).
+      specialize (H3 _ _ TR); cbn in H3.
+      next; right.
+      split.
+      * apply can_step_tau.
+        exists t', w'; auto.
+      * intros t_ w_ TR_.
+        rewrite ktrans_tau in TR_.
+        now apply H2.
+  Qed.
+
+  Lemma af_vis: forall (e: E) (k: encode e -> itree E X) (_: encode e) w φ,
+      (φ w \/ (not_done w /\ forall (x: encode e), <( {k x}, {Obs e x} |= AF now φ )>)) ->
+      <( {Vis e k}, w |= AF now φ )>.        
+  Proof.
+    intros.
+    destruct H as [H | [Hd H]].
+    - now next; left.
+    - next; right; next; split.
+      + now apply can_step_vis.
+      + intros t' w' TR'.
+        apply ktrans_vis in TR' as (? & -> & -> & ?).
+        apply H.
+  Qed.
+
+End BasicLemmas.
+
+Section AfIndLemma.
   Context {E: Type} {HE: Encode E} {X: Type}
-    (φ: itree E X -> World E -> Prop) {HP: Proper (equ X ==> eq ==> iff) φ}.
+    (φ: itree E X -> World E -> Prop).
   
   (*| [t |= AF φ] is semantic and requires double induction, on [AF] and inside it, in
   [ktrans]. Attempt to simplify to one induction with [AFInd] |*)
@@ -74,13 +114,54 @@ Section CtlITrees.
     - now apply AFIndBase.
   Qed.
 
-  Lemma af_afind {Hpr: @Productive E HE}
-                 {TauInv: forall (t: itree E X) w, φ t w  -> φ (Tau t) w}
-    : forall (t: itree E X) (w: World E),
-      AFInd t w <-> cau true (fun _ _ => True) φ t w.
+  (* This is a super useful lemma, it allows us to do induction on [AFInd]
+     instead of two inductions on [cau] and [trans] *)
+  Opaque Itree.stuck.
+  Lemma af_afind : forall (t: itree E X) (w: World E),
+       cau true (fun _ _ => True) φ t w -> AFInd t w.
   Proof.
-    split; intros; induction H.
-    (* -> *)
+    intros; induction H.
+    - now apply AFIndBase.
+    - destruct H0, H1; clear H H1.
+      destruct H0 as (t' & w' & TR).
+      cbn in TR.
+      dependent induction TR.
+      + observe_equ x.
+        eapply AFIndVis with (e:=e) (k:=k); auto.
+        intros v'.
+        apply H3; cbn.
+        rewrite <- x0.
+        apply KtransObs; auto.
+      + eapply AFIndTau with (u:=t0); auto.
+        eapply (IHTR) with (t':=t'); auto.
+        -- intros t_ w_ TR_.
+           apply H2; cbn.
+           rewrite <- x0.
+           now apply ktrans_tau.
+        -- intros t_ w_ TR_.
+           apply H3; cbn.
+           rewrite <- x0.
+           now apply ktrans_tau.
+      + apply AFIndDoneBase with (x:=x0); auto.
+        assert (TR_: [t, Pure] ↦ [Itree.stuck, Done x0]).
+        { cbn; rewrite <- x1; apply KtransDone; auto. }
+        specialize (H3 _ _ TR_).
+        now apply af_ind_stuck_done.
+      + apply AFIndFinishBase with (x:=x0); auto.
+        assert (TR_: [t, Obs e v] ↦ [Itree.stuck, Finish e v x0]).
+        { cbn; rewrite <- x1; apply KtransFinish; auto. }
+        specialize (H3 _ _ TR_).
+        now apply af_ind_stuck_finish.
+  Qed.
+  
+  (* -> *)
+  Lemma afind_af {Hpr: @Productive E HE}
+    {HP: Proper (equ X ==> eq ==> iff) φ}
+    {TauInv: forall (t: itree E X) w, φ t w  -> φ (Tau t) w}
+    : forall (t: itree E X) (w: World E),
+      AFInd t w -> cau true (fun _ _ => True) φ t w.
+  Proof.
+    intros; induction H.
     - now apply MatchA.
     - apply StepA; auto; split.
       + exists Itree.stuck, (Done x).
@@ -127,20 +208,127 @@ Section CtlITrees.
       + apply ktrans_vis in TR as (v & ? & -> & ?).
         rewrite H3.
         eapply H2.
-    - (* <- *)
-      now apply AFIndBase.
-    - destruct H0, H1; clear H H1.
-      destruct H0 as (t' & w' & TR).
+  Qed.
+End AfIndLemma.
+
+Section AfDoneIndLemma.
+  Context {E: Type} {HE: Encode E} {X: Type} (φ: X -> World E -> Prop).
+
+  Inductive AFDoneInd: itree E X -> World E -> Prop :=
+  | AFDoneDoneBase: forall t (x: X),
+      observe t = RetF x ->
+      φ x Pure ->
+      AFDoneInd t Pure
+  | AFDoneFinishBase: forall t (e: E) (v: encode e) (x: X),
+      observe t = RetF x ->
+      φ x (Obs e v) ->
+      AFDoneInd t (Obs e v)
+  | AFDoneIndTau: forall t u w,
+      observe t = TauF u ->
+      AFDoneInd u w ->
+      AFDoneInd t w
+  |AFDoneIndVis: forall (t: itree E X) w e k (_: encode e),
+      observe t = VisF e k ->
+      not_done w ->
+      (forall (v: encode e), AFDoneInd (k v) (Obs e v)) ->
+      AFDoneInd t w.
+
+  Global Instance proper_equ_afdoneind:
+    Proper (equ X ==> eq ==> iff) AFDoneInd.
+  Proof.
+    unfold Proper, respectful.
+    intros; subst; split; intros Hind.
+    - generalize dependent y.
+      induction Hind; intros.
+      + apply AFDoneDoneBase with x; auto.
+        rewrite <- H.
+        unfold equ in H.
+        step in H1; cbn in H1; dependent destruction H1; congruence.
+      + apply AFDoneFinishBase with x; auto.
+        rewrite <- H.
+        step in H1; cbn in H1; dependent destruction H1; congruence.
+      + unfold equ; step in H0; cbn in H0; rewrite H in H0.
+        dependent destruction H0.
+        apply IHHind in H0.
+        apply AFDoneIndTau with t2; congruence.
+      + unfold equ; step in H3; cbn in H3; rewrite H in H3.
+        dependent destruction H3.
+        eapply AFDoneIndVis with e k2; auto.
+        intros.
+        apply H2, H3.
+    - generalize dependent x.
+      induction Hind; intros.
+      + apply AFDoneDoneBase with x; auto.
+        rewrite <- H.
+        unfold equ in H.
+        step in H1; cbn in H1; dependent destruction H1; congruence.
+      + apply AFDoneFinishBase with x; auto.
+        rewrite <- H.
+        step in H1; cbn in H1; dependent destruction H1; congruence.
+      + unfold equ; step in H0; cbn in H0; rewrite H in H0.
+        dependent destruction H0.
+        apply IHHind in H0.
+        apply AFDoneIndTau with t1; congruence.
+      + unfold equ; step in H3; cbn in H3; rewrite H in H3.
+        dependent destruction H3.
+        eapply AFDoneIndVis with e k1; auto.
+        intros.
+        apply H2, H3.
+  Qed.
+
+  Lemma afdoneind_stuck: forall w,
+      ~ (AFDoneInd Itree.stuck w).
+  Proof.
+    intros * Hcontra.
+    dependent induction Hcontra; eauto.
+  Qed.
+
+  Lemma afdone_ind: forall (t: itree E X) w,
+      <( t, w |= AF AX done φ )> ->
+      AFDoneInd t w.
+  Proof.
+    intros; induction H.
+    - next in H.
+      destruct H as [(t' & w' & TR) H].
       cbn in TR.
       dependent induction TR.
-      + observe_equ x.
-        eapply AFIndVis with (e:=e) (k:=k); auto.
+      + eapply AFDoneIndVis; eauto.
         intros v'.
-        apply H3; cbn.
+        assert (TR: ktrans_ (observe t) w (observe (k v')) (Obs e v')).
+        { rewrite <- x0; apply ktrans_vis; exists v'; eauto. }
+        specialize (H1 _ _ TR).
+        rewrite ctl_done in H1.
+        inv H1.
+      + eapply AFDoneIndTau with (u:=t0); auto.
+        eapply IHTR; auto.
+        intros t_ w_ TR_.
+        apply H; cbn.
         rewrite <- x0.
-        apply KtransObs; auto.
-      + eapply AFIndTau with (u:=t0); auto.
-        eapply (IHTR HP) with (t':=t'); auto.
+        now apply ktrans_tau.
+      + eapply AFDoneDoneBase with (x:=x0); auto.
+        assert (TR: ktrans_ (observe t) Pure (observe Itree.stuck) (Done x0)).
+        { rewrite <- x1; econstructor; auto. }
+        specialize (H0 _ _ TR).
+        rewrite ctl_done in H0.
+        now dependent destruction H0.
+      + eapply AFDoneFinishBase with (x:=x0); auto.
+        assert (TR: ktrans_ (observe t) (Obs e v) (observe Itree.stuck) (Finish e v x0)).
+        { rewrite <- x1; econstructor; auto. }
+        specialize (H0 _ _ TR).
+        rewrite ctl_done in H0.
+        now dependent destruction H0.
+    -  destruct H0, H1; clear H H1.
+       destruct H0 as (t' & w' & TR).
+       cbn in TR.
+       dependent induction TR.
+       + observe_equ x.
+         eapply AFDoneIndVis with (e:=e) (k:=k); auto.
+         intros v'.
+         apply H3; cbn.
+         rewrite <- x0.
+         apply KtransObs; auto.
+      + eapply AFDoneIndTau with (u:=t0); auto.
+        eapply (IHTR) with (t':=t'); auto.
         -- intros t_ w_ TR_.
            apply H2; cbn.
            rewrite <- x0.
@@ -149,322 +337,109 @@ Section CtlITrees.
            apply H3; cbn.
            rewrite <- x0.
            now apply ktrans_tau.
-      + apply AFIndDoneBase with (x:=x0); auto.
-        assert (TR_: [t, Pure] ↦ [Itree.stuck, Done x0]).
-        { cbn; rewrite <- x1; apply KtransDone; auto. }
+      + apply AFDoneDoneBase with (x:=x0); auto.
+        assert (TR_: ktrans_ (observe t) Pure (observe Itree.stuck) (Done x0)).
+        { rewrite <- x1; apply KtransDone; auto. }
         specialize (H3 _ _ TR_).
-        now apply af_ind_stuck_done.
-      + apply AFIndFinishBase with (x:=x0); auto.
-        assert (TR_: [t, Obs e v] ↦ [Itree.stuck, Finish e v x0]).
-        { cbn; rewrite <- x1; apply KtransFinish; auto. }
+        now apply afdoneind_stuck in H3.
+      + apply AFDoneFinishBase with (x:=x0); auto.
+        assert (TR_: ktrans_ (observe t) (Obs e v) (observe Itree.stuck) (Finish e v x0)).
+        { rewrite <- x1; apply KtransFinish; auto. }
         specialize (H3 _ _ TR_).
-        now apply af_ind_stuck_finish.
-  Qed.
-  
-  Lemma ctl_af_tau: forall (t: itree E X) w φ,
-      <( t, w |= AF now φ )> -> 
-      <( {Tau t}, w |= AF (now φ) )>.
-  Proof.
-    intros.
-    unfold entailsF in H.
-    induction H.
-    - now next; left.
-    - Opaque entailsF.
-      destruct H0, H1; clear H H1.
-      destruct H0 as (t' & w' & TR).
-      specialize (H3 _ _ TR); cbn in H3.
-      next; right.
-      split.
-      * apply can_step_tau.
-        exists t', w'; auto.
-      * intros t_ w_ TR_.
-        rewrite ktrans_tau in TR_.
-        now apply H2.
+        now apply afdoneind_stuck in H3.
   Qed.
 
-  Lemma ctl_af_vis: forall (e: E) (k: encode e -> itree E X) (_: encode e) w φ,
-      (φ w \/ (not_done w /\ forall (x: encode e), <( {k x}, {Obs e x} |= AF now φ )>)) ->
-      <( {Vis e k}, w |= AF now φ )>.        
-  Proof.
-    intros.
-    destruct H as [H | [Hd H]].
-    - now next; left.
-    - next; right; next; split.
-      + now apply can_step_vis.
-      + intros t' w' TR'.
-        apply ktrans_vis in TR' as (? & -> & -> & ?).
-        apply H.
-  Qed.
-
-End CtlITrees.
+End AfDoneIndLemma.
 
 Section CtlAfBind.
   Context {E: Type} {HE: Encode E}.
 
-  Lemma ctl_stuck_obs_af{X}: forall (x: X) φ w,
-      return_eq X x w ->
-      ~ <( {Itree.stuck: itree E X}, w |= AF obs φ )>.
+  Lemma af_stuck{X}: forall φ w,
+      φ w <->
+      <( {Itree.stuck: itree E X}, w |= AF now φ )>.
   Proof.
-    intros * Hret Hcontra.
-    inv Hcontra.
-    - inv H; cbn in *; subst. 
-      destruct Hret; inv H.
-    - destruct H0 as ((? & ? & ?) & ?).
-      now apply ktrans_stuck in H0.
+    split; intros.
+    - next; left; auto.
+    - remember Itree.stuck as S. 
+      apply af_afind in H.
+      Transparent Itree.stuck.
+      induction H; subst; auto; cbn in *;
+        dependent destruction H; auto.      
   Qed.
 
-  Lemma ctl_obs_af_inv{X}: forall (t: itree E X) φ w,
-      <( t, w |= AF obs φ )> ->
-      not_done w.  
-  Proof.
-    intros * Haf.
-    next in Haf; destruct Haf; cbn in H.
-    - inv H. 
-      constructor.
-    - destruct H. 
-      destruct H as (t' & w' & TR).
-      now eapply ktrans_not_done with t t' w'.
-  Qed.
-  Hint Resolve ctl_obs_af_inv: ctl.
-
-  Theorem ctl_bind_af_l{X Y}: forall (t: itree E Y) (k: Y -> itree E X) φ w,
+  Theorem af_bind_obs{X Y}: forall (t: itree E Y) (k: Y -> itree E X) φ w,
       <( t, w |= AF obs φ )> ->
       <( {x <- t ;; k x}, w |= AF obs φ )>.
   Proof.
     intros * Haf.
-    revert X k.
+    apply af_afind in Haf.
+    revert X k.    
     induction Haf; intros; subst. 
-    - (* MatchA *)
-      next; left; cbn.
-      apply H.
-    - (* StepA *)
-      destruct H0, H1; clear H H0.
-      destruct H1 as (te & we & TR); cbn in TR.
-      dependent destruction TR.
-      + next; right; next; split. 
-        * apply can_step_bind_l with t0 (Obs e v); cbn. 
-          -- rewrite <- x0.
-             now apply KtransObs.
-          -- constructor.
-        * intros k' w' TR'.
-          apply ktrans_bind_inv in TR'
-              as [(t' & TR' & Hd & ?) |
-               [(y & TRr & -> & TRk) |
-                 (e' & v' & x' & TRr & -> & TRk)]].
-          -- rewrite H1.
-             apply (H3 t' w' TR').
-          -- specialize (H2 Itree.stuck (Done y) TRr).
-             Transparent entailsF.
-             apply ctl_stuck_obs_af with (x:=y) in H2; intuition.
-          -- specialize (H2 Itree.stuck (Finish e' v' x') TRr).
-             apply ctl_stuck_obs_af with (x:=x') in H2; intuition.
-      + observe_equ x0.
-        rewrite Eqt.
-        assert (TRtau: ktrans_ (observe t) w (observe t') we).
-        { rewrite x0; now apply KtransTau. }        
-        next; right; next; split. 
-        * eapply can_step_bind_l; cbn.
-          apply KtransTau; eauto.
-          specialize (H3 t' we TRtau _ k); cbn in H3.        
-          now apply ctl_obs_af_inv in H3.
-        * intros k' w' TR'.
-          apply ktrans_bind_inv in TR'
-              as [(t_ & TR_ & Hd & ?) |
-                   [(y & TRt' & -> & TRk) |
-                     (e' & v' & x' & TRr & -> & TRk)]].
-          -- rewrite H.
-             specialize (H3 t_ w'); cbn in H2.
-             rewrite ktrans_tau in TR_.
-             apply H3; cbn.
-             rewrite x0.
-             now apply ktrans_tau.
-          -- cbn in TRt'.
-             rewrite <- x0 in TRt'.
-             specialize (H2 Itree.stuck (Done y) TRt'); cbn in H2.             
-             Transparent entailsF.
-             eapply ctl_stuck_obs_af with (x:=y) in H2; intuition.
-          -- cbn in TRr.
-             rewrite <- x0 in TRr.
-             specialize (H2 Itree.stuck (Finish e' v' x') TRr); cbn in H2.             
-             Transparent entailsF.
-             eapply ctl_stuck_obs_af with (x:=x') in H2; intuition.
-      + assert (TRt: ktrans_ (observe t) Pure (observe Itree.stuck) (Done x0)).
-        { rewrite <- x1; apply KtransDone; reflexivity. }.
-        specialize (H3 Itree.stuck (Done x0) TRt _ k); cbn in H3.
-        apply ctl_obs_af_inv in H3; inv H3.
-      + assert (TRt: ktrans_ (observe t) (Obs e v) (observe Itree.stuck) (Finish e v x0)).
-        { rewrite <- x1; apply KtransFinish; reflexivity. }.
-        specialize (H3 Itree.stuck (Finish e v x0) TRt _ k).
-        apply ctl_obs_af_inv in H3; inv H3.
-  Qed.
-
-  Lemma ctl_return_af_inv{X}: forall (t: itree E X) w (r: X),
-      <( t, w |= AF return r )> ->
-      return_eq X r w \/ ALeaf (eq r) t.
-  Proof.
-    intros.
-    induction H.
-    - left; auto.
-    - destruct H0, H1; clear H H1.
-      destruct H0 as (t' & w' & TR'); cbn.
-      generalize dependent r.      
-      ktrans_ind TR'; intros.
-      + right; eapply ALeafVis.
-        * now rewrite x0.
-        * intro x'.          
-          assert (TR_: [t, w] ↦ [k x', Obs e x']).
-          { cbn.
-            rewrite <- x0.
-            eapply KtransObs; auto.
-          }.
-          destruct (H3 _ _ TR_); cbn in H1.
-          -- destruct H1; inv H1.
-          -- auto.
-      + edestruct IHTR' with (t':=t'); eauto.
-          -- intros t_ w_ TR_.
-             apply H2; cbn.
-             rewrite <- x0; now apply KtransTau.
-          -- intros t_ w_ TR_.
-             apply H3; cbn.
-             rewrite <- x0; now apply KtransTau.
-          -- right.
-             eapply ALeafTau.
-             ++ now rewrite x0.
-             ++ auto.
-      + right; eapply ALeafRet.
-        assert (TR_: [t, Pure] ↦ [Itree.stuck, Done x0]).
-        { cbn.
-          rewrite <- x1.
-          replace (TauF Itree.stuck) with (observe Itree.stuck (X:=X)) by reflexivity.
-          apply KtransDone; auto.
-        }
-        destruct (H3 _ _ TR_); cbn in H0.
-        * destruct H0; dependent destruction H0.
-          now rewrite x1.
-        * now apply ALeaf_stuck in H0.
-        * reflexivity.
-      + right; eapply ALeafRet.
-        assert (TR_: [t, Obs e v] ↦ [Itree.stuck, Finish e v x0]).
-        { cbn.
-          rewrite <- x1.
-          replace (TauF Itree.stuck) with (observe Itree.stuck (X:=X)) by reflexivity.
-          apply KtransFinish; auto.
-        }
-        destruct (H3 _ _ TR_); cbn in H0.        
-        * destruct H0; dependent destruction H0.
-          now rewrite x1.
-        * now apply ALeaf_stuck in H0.
-        * reflexivity.
+    - (* Base *)
+      next; left; cbn; apply H.
+    - (* Done *)
+      destruct H0 as (? & ? & ? & ?).
+      inv H0.
+    - (* Finish *)
+      destruct H0 as (? & ? & ? & ?).
+      inv H0.
+    - (* Tau *)
+      observe_equ H.
+      rewrite Eqt, bind_tau.
+      apply af_tau; eauto.
+    - (* Vis *)
+      observe_equ H.
+      rewrite Eqt, bind_vis.
+      apply af_vis; eauto.
   Qed.
 
   Lemma can_step_bind_r{X Y} {HP: Productive E}:
-    forall (t: itree E Y) (k: Y -> itree E X) w (r: Y),      
-      <( t, w |= AF return r )> ->
-      can_step (k r) w ->
+    forall (t: itree E Y) (k: Y -> itree E X) w R,      
+      <( t, w |= AF AX done R )> ->
+      (forall y w, R y w -> can_step (k y) w) ->
       can_step (x <- t ;; k x) w.
   Proof.    
     intros.
-    apply ctl_return_af_inv in H as [H|H].
-    - destruct H; inv H. (* (kr, w) can step, so w != done *)
-      + apply can_step_not_done in H0; inv H0.
-      + apply can_step_not_done in H0; inv H0. 
-    - revert w k H0.
-      dependent induction H; intros;
-        observe_equ H; rewrite Eqt, ?bind_ret_l; subst.
-      + exact H1.
-      + rewrite bind_tau.
-        eapply can_step_tau.
-        now apply IHALeaf.
-      + rewrite bind_vis.
-        apply can_step_vis.
-        * (* Indeed, [x <- Vis (e: void) ;; k x]
-             does not step, need [Productive E] *)
-          apply HP.
-        * now apply can_step_not_done in H2. 
+    apply afdone_ind in H.
+    generalize dependent k.
+    induction H; intros; observe_equ H; rewrite Eqt.
+    - (* Done x *)
+      rewrite bind_ret_l.
+      now apply H1.
+    - (* Finish *)
+      rewrite bind_ret_l.
+      now apply H1.
+    - (* Tau *)
+      rewrite bind_tau.
+      apply can_step_tau; eauto.
+    - (* Vis *)
+      rewrite bind_vis.
+      apply can_step_vis; auto.
   Qed.
   Hint Resolve can_step_bind_r: ctl.
 
-   Theorem ctl_bind_af_finish{X Y} {HP: Productive E}:
+  Theorem af_bind_r{X Y} {HP: Productive E}:
     forall (t: itree E Y) (k: Y -> itree E X) w φ R,
-      <( t, w |= AF finish R )> ->
-      (forall (e: E) (v: encode e) (y: Y), R e v y -> <( {k y}, {Obs e v} |= AF now φ )>) ->
+      <( t, w |= AF AX done R )> ->
+      (forall (y: Y) w, R y w -> <( {k y}, w |= AF now φ )>) ->
       <( {x <- t ;; k x}, w |= AF now φ )>.
   Proof.
     intros.
+    apply afdone_ind in H.
     revert H0.
     generalize dependent φ.
     generalize dependent k.
-    induction H; intros; cbn in H.
-    - inv H.
-     
-    - destruct H0, H1; clear H H1.
-      destruct H0 as (t' & w' & TR'); cbn.
-      generalize dependent r.      
-      ktrans_ind TR'; intros.
-      
-    apply ctl_return_af_inv in H as [H|H].
-    - specialize (H0 w).
-      destruct H; inv H; inv H0.
-      + now next; left.
-      + destruct H1.
-        apply can_step_not_done in H0; inv H0. 
-      + now next; left.
-      + destruct H1.
-        apply can_step_not_done in H0; inv H0.
-    - generalize dependent w.
-      revert H0.
-      dependent induction H; intros; observe_equ H.
-      + now rewrite Eqt, bind_ret_l.
-      + rewrite Eqt, bind_tau.
-        apply ctl_af_tau.
-        now apply IHALeaf.
-      + rewrite Eqt, bind_vis.
-        apply ctl_af_vis.
-        * apply HP.
-        * destruct (not_done_dec w).
-          -- right; split; auto.
-          -- left.
-             specialize (H2 w).
-             auto.
-             apply H1.
-             (* Here, AF [return r] says nothing about the return value
-                of [w], need a more specific predicate like [finish ψ] (see slack) *)
-             apply H1.
-  Admitted.
+    induction H; intros; observe_equ H; rewrite Eqt.
+    - (* Done *)
+      rewrite bind_ret_l; eauto.
+    - (* Finish *)
+      rewrite bind_ret_l; eauto.
+    - (* Tau *)
+      rewrite bind_tau.
+      apply af_tau; eauto.
+    - (* Vis *)
+      rewrite bind_vis.
+      apply af_vis; eauto.
+  Qed.
   
-  Theorem ctl_bind_af_r{X Y} {HP: Productive E}:
-    forall (t: itree E Y) (k: Y -> itree E X) w φ
-      (ψ: forall (e: E), encode e -> Y -> Prop),
-      <( {(t, w)} |= AF finish ψ )> ->
-      (forall (e: E) (v: encode e) (r: Y),
-          ψ e v r -> <( {(k r, Obs e v)} |= AF now φ )>) ->
-      <( {(x <- t ;; k x, w)} |= AF now φ )>.
-  Proof.
-    intros.
-    apply ctl_return_af_inv in H as [H|H].
-    - inv H; inv H0.
-      + now next; left.
-      + destruct H1.
-        apply can_step_not_done in H0; inv H0. 
-      + now next; left.
-      + destruct H1.
-        apply can_step_not_done in H0; inv H0.
-    - generalize dependent w.
-      dependent induction H; intros; observe_equ H.
-      + now rewrite Eqt, bind_ret_l.
-      + rewrite Eqt, bind_tau.
-        apply ctl_af_tau.
-        now apply IHALeaf.
-      + rewrite Eqt, bind_vis.
-        apply ctl_af_vis.
-        * apply HP.
-        * destruct (not_done_dec w).
-          -- right; split; auto.
-             intro x'.
-             apply H1.
-             (* Here, AF [return r] says nothing about the return value
-                of [w], need a more specific predicate like [finish ψ] (see slack) *)
-             apply H1.
-  Admitted.
-
-End CtlITrees.
+End CtlAfBind.
